unify ch03/ex03 and ch04/ex02 with inlining

chapter04-inv/solutions/exercise02_solution.dfy
@@ -7,96 +7,38 @@
 // You are welcome to prove correct your own model from chapter03,
 // but note that may be too hard or too easy if your spec is broken.
 
-datatype ServerGrant = Unlocked | Client(id: nat)
-
-datatype ClientRecord = Released | Acquired
-
-datatype Variables = Variables(server: ServerGrant, clients: seq<ClientRecord>)
-
-predicate Init(v: Variables) {
-  && v.server.Unlocked?
-  && forall i | 0 <= i < |v.clients| :: v.clients[i].Released?
-}
-
-predicate Acquire(v: Variables, v':Variables, id:int) {
-  && 0 <= id < |v.clients|
-
-  // Enabling condition: The server checks its local state.
-  && v.server.Unlocked?
-
-  // Update the server state.
-  && v'.server == Client(id)
-
-  // Update the client that acquired.
-  && |v'.clients| == |v.clients|  // Don't lose track of any clients.
-  && ( forall i | 0 <= i < |v.clients| ::
-      v'.clients[i] == if i == id then Acquired else v.clients[i] )
-}
-
-predicate Release(v: Variables, v':Variables, id:int) {
-  && 0 <= id < |v.clients|
-
-  // Enabling condition: The client trying to release checks its local state.
-  && v.clients[id].Acquired?
-
-  // Update the server state.
-  && v'.server.Unlocked?
-
-  // Update the client that released.
-  && |v'.clients| == |v.clients|  // Don't lose track of any clients.
-  && ( forall i | 0 <= i < |v.clients| ::
-      v'.clients[i] == if i == id then Released else v.clients[i] )
-}
-
-datatype Step = AcquireStep(id:int) | ReleaseStep(id:int)
-
-predicate NextStep(v:Variables, v':Variables, step:Step) {
-  match step {
-    case AcquireStep(toClient) => Acquire(v, v', toClient)
-    case ReleaseStep(fromClient) => Release(v, v', fromClient)
-  }
-}
-
-predicate Next(v:Variables, v':Variables) {
-  exists step :: NextStep(v, v', step)
-}
-
-predicate Safety(v:Variables) {
-  // No two clients have the lock simultaneously.
-  forall i,j ::
-    (&& 0 <= i < |v.clients|
-    && 0 <= j < |v.clients|
-    && v.clients[i].Acquired?
-    && v.clients[j].Acquired?) ==> i == j
-}
+//#inline "../../chapter03-sm/solutions/exercise03_solution.dfy"
+//#start-elide
+include "../../chapter03-sm/solutions/exercise03_solution.dfy"
+//#end-elide
 
 //#start-elide
 // Safety doesn't care what server thinks, but to get an *inductive* invariant,
 // we need to ensure the server doesn't fall out of sync with the clients'
 // beliefs.
-predicate ServerAgreesClients(v:Variables) {
+predicate ServerAgreesClients(c:Constants, v:Variables) {
   v.server.Unlocked? <==> (forall id | 0 <= id < |v.clients| :: v.clients[id].Released?)
 }
 
 //#end-elide
-predicate Inv(v:Variables) {
-//#exercise  true  // probably not strong enough. :v)
+predicate Inv(c:Constants, v:Variables) {
+//#exercise  true  // Replace me: probably not strong enough. :v)
 //#start-elide
-  && Safety(v)
-  && ServerAgreesClients(v)
+  && Safety(c, v)
+  && ServerAgreesClients(c, v)
 //#end-elide
 }
 
 // Here's your obligation. Probably easiest to break this up into three
 // lemmas, each P==>Q becomes requires P ensures Q.
-lemma SafetyTheorem(v:Variables, v':Variables)
-  ensures Init(v) ==> Inv(v)
-  ensures Inv(v) && Next(v, v') ==> Inv(v')
-  ensures Inv(v) ==> Safety(v)
+lemma SafetyTheorem(c:Constants, v:Variables, v':Variables)
+  ensures Init(c, v) ==> Inv(c, v)
+  ensures Inv(c, v) && Next(c, v, v') ==> Inv(c, v')
+  ensures Inv(c, v) ==> Safety(c, v)
 {
 //#start-elide
-  if Inv(v) && Next(v, v') {
-    var step :| NextStep(v, v', step);        // give a variable name ("step") to what happened in Next
+  if Inv(c, v) && Next(c, v, v') {
+    var step :| NextStep(c, v, v', step);        // give a variable name ("step") to what happened in Next
     if step.AcquireStep? {                    // case analysis
 //      assert !v'.server.Unlocked?;
       assert !v'.clients[step.id].Released?;  // witness to exist (!forall in ServerAgreesClient)
